---
title: "Variance of a Binomial"
author: "Evan Blosser"
date: "`r Sys.Date()`"
output: 
  html_document: 
    toc: yes
    toc_float: yes
---

```{r setup, include=FALSE}
knitr::opts_chunk$set(echo = TRUE, message = FALSE)
```

# Introduction

We have learnt that the MGF for a binomial random variable is:

$$M_X(t) = (q+pe^t)^n $$

Where $X\sim Bin(n,p)$

# Tasks

Using the moment generating function above prove that 

$$\sigma^2 = npq$$

by answering the tasks below. 
You may use $\LaTeX$ to construct the proof OR write the proof on paper and incluse using `![](){}`.

## Task 1

Start with 

$$
\begin{eqnarray}
E(X) &=& \left . \frac{d M_X(t)}{dt}\right |_{t=0}\\
     &=&   \big(  n(q+pe^t)^{n-1}pe^t  \big) |_{t=0}\\
     &=& \big(  n(q+pe^{(0)})^{n-1}pe^{(0)}  \big)\\
     &=& n(q+p(1))^{n-1}p(1)\\
     &=& n(q+p)^{n-1}p\\
     let: (q+p) &=& 1\\
E(X) &=& n(1)^{n-1}p = \mu\\
\\
thus:\\
     \mu &=& np
\end{eqnarray}
$$
Thus, we find that $E(X) = np$.

## Task 2

Now find $E(X^2)$

$$
\begin{eqnarray}
E(X^2) &=& \left . \frac{d^2 M_X(t)}{dt^2}\right |_{t=0}\\
       &=& \frac{d}{dt} \bigg[\big(  n(q+pe^t)^{n-1}pe^t  \big) \bigg|_{t=0}\\
       &=& np\frac{d}{dt} \bigg[\big(  (q+pe^t)^{n-1}e^t  \big) \bigg|_{t=0}\\
       &=& np \bigg[\big( (n-1)pe^t(q+pe^t)^{n-2}e^t + (q+pe^t)^{n-1}e^t \big) \bigg|_{t=0}\\
       &=& np \bigg[ (n-1)pe^{(0)}(q+pe^{(0)})^{n-2}e^{(0)} + (q+pe^{(0)})^{n-1}e^{(0)}  \bigg]\\
       &=& np \bigg[ (n-1)p(1)(q+p(1))^{n-2}(1) + (q+p(1))^{n-1}(1)  \bigg]\\
       &=& np \bigg[ (n-1)p(q+p)^{n-2} + (q+p)^{n-1}  \bigg]\\
       &=& np \bigg[ (n-1)p(1)^{n-2} + (1)^{n-1}  \bigg]\\
       &=& np \big[ (n-1)p + 1 \big]\\
       &=& np(np-p+1)\\
       where: q &=& 1- p\\
E(X^2) &=& np(np+q)\\
       &=& n^2p^2 + npq
\end{eqnarray}
$$

## Task 3

Find $\sigma^2$ Using the formula $\sigma^2 =E(X^2)-\mu^2$

previously it was found that:
$$
\begin{eqnarray}
\mu   &=& np\\
E(X^2) &=& n^2p^2 + npq
\end{eqnarray}
$$
Thus:
$$
\begin{eqnarray}
\sigma^2  &=& E(X^2)-\mu^2\\
          &=& n^2p^2 + npq - (np)^2\\
          &=& n^2p^2 + npq - n^2p^2\\
          &=& npq
\end{eqnarray}
$$
Finally we prove that: $\sigma^2  = npq$



